Updated proof of soundness for E3. Proved initial state case with some help from sledgehammer.

src/E3.thy
@@ -41,11 +41,11 @@ definition add_todo :: "
 
 definition pop_todo :: "
 ('set_todo_done,'map_blocked_key,'map_complete_key,'map_sym_sym_int_int,'map_tm_int) ty_loop2
-=> (('set_todo_done,'map_blocked_key,'map_complete_key,'map_sym_sym_int_int,'map_tm_int) ty_loop2 * item)" where
+=> (('set_todo_done,'map_blocked_key,'map_complete_key,'map_sym_sym_int_int,'map_tm_int) ty_loop2 * item) option" where
 "pop_todo s0 = (
   case (todo5 s0) of
-    [] => (failwith ''pop_todo'')
-  | x#xs => (s0 (| todo5 :=xs |),x))"
+    [] => None (*(failwith ''pop_todo'') *)
+  | x#xs => Some (s0 (| todo5 :=xs |),x))"
 
 
 definition cut :: "
@@ -74,107 +74,110 @@ definition loop2 :: "
 => ('set_todo_done,'map_blocked_key,'map_complete_key,'map_sym_sym_int_int,'map_tm_int) ty_loop2" where
 "loop2 ctxt s0 == (
   let ops = (item_ops5 ctxt) in
-  let (s0,itm0) = pop_todo s0 in
+  case pop_todo s0 of
+    Some (s0, itm0) \<Rightarrow>
+  (*let (s0,itm0) = pop_todo s0 in *)
   (* FIXME add a case construct rather than dests *)
-  case (dest_item ops) itm0 of
-    NTITM nitm => (
-      let complete = (b2_nil ops) nitm in
-      case complete of
-        True => (
-          let citm = (mk_sym_coord ops) ((nt2 ops) nitm, (nt_dot_i9 ops) nitm, (nt_dot_j9 ops) nitm) in
-          let k = ((sym_dot_i9 ops) citm (* FIXME could be from dot_i9 nitm *),(ops |> sym6) citm) in
-          (* FIXME check whether citm has already been done? *)
-          (*let citms = ctxt.maps.map_complete_key.find2 k s0.complete5 in *)
-          case False (* ctxt.sets.set_sym_item.std_mem citm citms *) of (* FIXME this optimization didn't buy much *)
-            True => s0
-          | False => (
-              (* let bitms = ctxt.maps.map_blocked_key.find2 k s0.blocked5 in *)
-              let f1 = % bitm s1. cut ctxt bitm citm s1 in
-              (* O(n. ln n) *)
-              (* let s0 = ctxt.sets.set_nt_item.fold f1 bitms s0 in *)
-              let s0 = (ctxt |> maps |> map_blocked_key |> mbk_fold_cod) k f1 (s0 |> blocked5) s0 in
-              let s0 = s0 (|
-                        complete5:=((ctxt |> maps |> map_complete_key |> mck_add_cod) k citm (s0 |> complete5)) |)
-              in
-              (* we also update the oracle at this ponat  FIXME this appears very costly *)
-              let f2 = % bitm s1. s1 (| oracle5:=(update_oracle ctxt (s1 |> oracle5) (bitm,(ops |> sym_dot_j9) citm)) |) in
-              (* O(n. ln n) *)
-              let s0 = (ctxt |> maps |> map_blocked_key |> mbk_fold_cod) k f2 (s0 |> blocked5) s0 in
-              s0))
-      | False => (
-          let bitm = nitm in
-          let sym = (ops |> hd_b2) bitm in
-          let k = ((ops |> nt_dot_j9) bitm,sym) in
-          (* let bitms = ctxt.maps.map_blocked_key.find2 k s0.blocked5 in *)
-          let new_key = (ctxt |> maps |> map_blocked_key |> mbk_cod_empty) k (s0 |> blocked5) in
-          let s0 = s0 (|
-                    blocked5:=((ctxt |> maps |> map_blocked_key |> mbk_add_cod) k bitm (s0 |> blocked5)) |)                                        
-          in    
-
-          (* we should also process the blocked item against the relevant complete items *)
-          (* let citms = ctxt.maps.map_complete_key.find2 k s0.complete5 in *)
-          let f3 = % citm s1. cut ctxt bitm citm s1 in
-          (* O(n. ln n) *)
-          let s0 = (ctxt |> maps |> map_complete_key |> mck_fold_cod) k f3 (s0 |> complete5) s0 in
-          (* we also update the oracle at this ponat; FIXME this appears very costly *)
-          let f4 = % citm s1. s1 (| oracle5:=(update_oracle ctxt (s1 |> oracle5) (bitm,(ops |> sym_dot_j9) citm)) |) in
-          (* O(n. ln n) *)
-          let s0 = (ctxt |> maps |> map_complete_key |> mck_fold_cod) k f4 (s0 |> complete5) s0 in                                                 
-
-          (* the invariant should be: if (j,nt) is nonempty then all                                                                               
-             nt items for j are already in set_todo_done; if (j,tm) is                                                                             
-             nonempty then all tmitems for j are already in                                                                                        
-             set_todo_done *)
-          if new_key then (
-            case (ops |> sym_case) sym of
-              NT nt => (
-                let rs = (ops |> nt_items_for_nt) nt ((ctxt |> string5), (ops |> nt_dot_i9) nitm, (ops |> nt_dot_j9) nitm) in
-                let f1 = (% s1 pnitm.
-                  let nitm = (ops |> mk_item) (NTITM pnitm) in
-                  if ((ctxt |> sets|>set_todo_done|>std_mem) nitm (s1|>todo_done5)) then s1 else
-                    add_todo ctxt s1 nitm)
+    case (dest_item ops) itm0 of
+      NTITM nitm => (
+        let complete = (b2_nil ops) nitm in
+        case complete of
+          True => (
+            let citm = (mk_sym_coord ops) ((nt2 ops) nitm, (nt_dot_i9 ops) nitm, (nt_dot_j9 ops) nitm) in
+            let k = ((sym_dot_i9 ops) citm (* FIXME could be from dot_i9 nitm *),(ops |> sym6) citm) in
+            (* FIXME check whether citm has already been done? *)
+            (*let citms = ctxt.maps.map_complete_key.find2 k s0.complete5 in *)
+            case False (* ctxt.sets.set_sym_item.std_mem citm citms *) of (* FIXME this optimization didn't buy much *)
+              True => s0
+            | False => (
+                (* let bitms = ctxt.maps.map_blocked_key.find2 k s0.blocked5 in *)
+                let f1 = % bitm s1. cut ctxt bitm citm s1 in
+                (* O(n. ln n) *)
+                (* let s0 = ctxt.sets.set_nt_item.fold f1 bitms s0 in *)
+                let s0 = (ctxt |> maps |> map_blocked_key |> mbk_fold_cod) k f1 (s0 |> blocked5) s0 in
+                let s0 = s0 (|
+                          complete5:=((ctxt |> maps |> map_complete_key |> mck_add_cod) k citm (s0 |> complete5)) |)
                 in
-                let s0 = List.foldl f1 s0 rs in
-                s0)
-            | TM tm => (                                                                                                                           
-                let titm = (ops|>mk_item) (TMITM((ops|>mk_tm_coord) (tm,(ops|>nt_dot_j9) nitm))) in
-                if ((ctxt|>sets|>set_todo_done|>std_mem) titm (s0|>todo_done5)) then s0 else
-                  add_todo ctxt s0 titm))
-          else
-            s0 
-       ))
-  | TMITM titm => (
-      let tm = (ops|>tm5) titm in
-      let p = (ops|>p_of_tm) tm in
-      let i = (ops|>tm_dot_i9) titm in
-      let rs = p (ctxt|>string5,i,ctxt|>length5) in                                                                                                
-      let sym = (ops|>sym_of_tm) tm in
-      let k = (i,sym) in                                                                                                                           
-      (* lots of new complete items, so complete5 must be updated, but we must also process blocked *)
-      (* let bitms = ctxt.maps.map_blocked_key.find2 k s0.blocked5 in *)
-      (* update complete set *)
-      let f5 = % s1 j. (                                                                                                                           
-        let citm = (ops|>mk_sym_coord) (sym,i,j) in
-        s1 (| complete5:=((ctxt|>maps|>map_complete_key|>mck_add_cod) k citm (s1|>complete5)) |))
-      in
-      let s0 = List.foldl f5 s0 rs in
-      let f8 = % s1 j. (
-        let i = ((ops|>tm_dot_i9) titm) in
-        let citm = (ops|>mk_sym_coord) (sym,i,j) in
-        let f6 = % bitm s1. cut ctxt bitm citm s1 in
-        (* O(n. ln n) *)
-        (* let s1 = ctxt.sets.set_nt_item.fold f1 bitms s1 in *)
-        let s1 = (ctxt|>maps|>map_blocked_key|>mbk_fold_cod) k f6 (s1|>blocked5) s1 in     
-        (* we also update the oracle at this point *)
-        let f7 = % bitm s1. s1 (| oracle5:=(update_oracle ctxt (s1|>oracle5) (bitm,(ops|>sym_dot_j9) citm)) |) in
-        (* O(n. ln n) *)
-        let s1 = (ctxt|>maps|>map_blocked_key|>mbk_fold_cod) k f7 (s1|>blocked5) s1 in
-        (* and the tmoracle *)
-        let s1 = s1 (| tmoracle5:=(update_tmoracle ctxt (s1|>tmoracle5) (tm,i,j)) |) in                                                            
-       s1)
-      in
-      let s0 = List.foldl f8 s0 rs in 
-      s0) (* FIXME todo *)
+                (* we also update the oracle at this ponat  FIXME this appears very costly *)
+                let f2 = % bitm s1. s1 (| oracle5:=(update_oracle ctxt (s1 |> oracle5) (bitm,(ops |> sym_dot_j9) citm)) |) in
+                (* O(n. ln n) *)
+                let s0 = (ctxt |> maps |> map_blocked_key |> mbk_fold_cod) k f2 (s0 |> blocked5) s0 in
+                s0))
+         | False => (
+            let bitm = nitm in
+            let sym = (ops |> hd_b2) bitm in
+            let k = ((ops |> nt_dot_j9) bitm,sym) in
+            (* let bitms = ctxt.maps.map_blocked_key.find2 k s0.blocked5 in *)
+            let new_key = (ctxt |> maps |> map_blocked_key |> mbk_cod_empty) k (s0 |> blocked5) in
+            let s0 = s0 (|
+                    blocked5:=((ctxt |> maps |> map_blocked_key |> mbk_add_cod) k bitm (s0 |> blocked5)) |)                                        
+            in    
+
+            (* we should also process the blocked item against the relevant complete items *)
+            (* let citms = ctxt.maps.map_complete_key.find2 k s0.complete5 in *)
+            let f3 = % citm s1. cut ctxt bitm citm s1 in
+            (* O(n. ln n) *)
+            let s0 = (ctxt |> maps |> map_complete_key |> mck_fold_cod) k f3 (s0 |> complete5) s0 in
+            (* we also update the oracle at this ponat; FIXME this appears very costly *)
+            let f4 = % citm s1. s1 (| oracle5:=(update_oracle ctxt (s1 |> oracle5) (bitm,(ops |> sym_dot_j9) citm)) |) in
+            (* O(n. ln n) *)
+            let s0 = (ctxt |> maps |> map_complete_key |> mck_fold_cod) k f4 (s0 |> complete5) s0 in                                                 
+
+            (* the invariant should be: if (j,nt) is nonempty then all                                                                               
+              nt items for j are already in set_todo_done; if (j,tm) is                                                                             
+              nonempty then all tmitems for j are already in                                                                                        
+              set_todo_done *)
+            if new_key then (
+              case (ops |> sym_case) sym of
+                NT nt => (
+                  let rs = (ops |> nt_items_for_nt) nt ((ctxt |> string5), (ops |> nt_dot_i9) nitm, (ops |> nt_dot_j9) nitm) in
+                  let f1 = (% s1 pnitm.
+                    let nitm = (ops |> mk_item) (NTITM pnitm) in
+                    if ((ctxt |> sets|>set_todo_done|>std_mem) nitm (s1|>todo_done5)) then s1 else
+                      add_todo ctxt s1 nitm)
+                  in
+                  let s0 = List.foldl f1 s0 rs in
+                  s0)
+              | TM tm => (                                                                                                                           
+                  let titm = (ops|>mk_item) (TMITM((ops|>mk_tm_coord) (tm,(ops|>nt_dot_j9) nitm))) in
+                  if ((ctxt|>sets|>set_todo_done|>std_mem) titm (s0|>todo_done5)) then s0 else
+                    add_todo ctxt s0 titm))
+            else
+              s0 
+        ))
+   | TMITM titm => (
+        let tm = (ops|>tm5) titm in
+        let p = (ops|>p_of_tm) tm in
+        let i = (ops|>tm_dot_i9) titm in
+        let rs = p (ctxt|>string5,i,ctxt|>length5) in                                                                                                
+        let sym = (ops|>sym_of_tm) tm in
+        let k = (i,sym) in                                                                                                                           
+        (* lots of new complete items, so complete5 must be updated, but we must also process blocked *)
+        (* let bitms = ctxt.maps.map_blocked_key.find2 k s0.blocked5 in *)
+        (* update complete set *)
+        let f5 = % s1 j. (                                                                                                                           
+          let citm = (ops|>mk_sym_coord) (sym,i,j) in
+          s1 (| complete5:=((ctxt|>maps|>map_complete_key|>mck_add_cod) k citm (s1|>complete5)) |))
+        in
+        let s0 = List.foldl f5 s0 rs in
+        let f8 = % s1 j. (
+          let i = ((ops|>tm_dot_i9) titm) in
+          let citm = (ops|>mk_sym_coord) (sym,i,j) in
+          let f6 = % bitm s1. cut ctxt bitm citm s1 in
+          (* O(n. ln n) *)
+          (* let s1 = ctxt.sets.set_nt_item.fold f1 bitms s1 in *)
+          let s1 = (ctxt|>maps|>map_blocked_key|>mbk_fold_cod) k f6 (s1|>blocked5) s1 in     
+          (* we also update the oracle at this point *)
+          let f7 = % bitm s1. s1 (| oracle5:=(update_oracle ctxt (s1|>oracle5) (bitm,(ops|>sym_dot_j9) citm)) |) in
+          (* O(n. ln n) *)
+          let s1 = (ctxt|>maps|>map_blocked_key|>mbk_fold_cod) k f7 (s1|>blocked5) s1 in
+          (* and the tmoracle *)
+          let s1 = s1 (| tmoracle5:=(update_tmoracle ctxt (s1|>tmoracle5) (tm,i,j)) |) in                                                            
+        s1)
+        in
+        let s0 = List.foldl f8 s0 rs in 
+        s0)
+  | None \<Rightarrow> s0  (* FIXME todo *)
 )
 "
 
